equivalence proof prior cleanup

src/Util/FisherYates/Implementation.dfy
@@ -5,19 +5,77 @@
 
 module FisherYates.Implementation {
   import Interface
+  import Monad
+  import Model
+  import Uniform
 
   trait {:termination false} Trait extends Interface.Trait {
 
-    method Shuffle<T>(a: array<T>)
+    method {:vcs_split_on_every_assert} Shuffle<T>(a: array<T>)
       decreases *
-      modifies this, a
+      modifies `s, a
+      ensures Model.Shuffle(old(a[..]))(old(s)) == Monad.Result(a[..], s)
     {
+      ghost var prevASeq := a[..];
+      ghost var prevI := 0;
+      ghost var prevS := s;
       if a.Length > 1 {
-        for i := 0 to a.Length - 1 {
+        var i := 0;
+        while i < a.Length - 1
+          decreases a.Length - 1 - i
+          invariant prevI == if i == 0 then i else i - 1
+          invariant prevI <= |prevASeq|
+          invariant i <= |a[..]|
+          invariant i <= a.Length - 1
+          invariant |prevASeq| == |a[..]| == a.Length
+          invariant Model.Shuffle(old(a[..]))(old(s)) == Model.Shuffle(prevASeq, prevI)(prevS)
+          invariant Model.Shuffle(prevASeq, prevI)(prevS) == Model.Shuffle(a[..], i)(s)
+        {
+          prevI := i;
+          prevASeq := a[..];
+          prevS := s;
           var j := UniformIntervalSample(i, a.Length);
-          a[i], a[j] := a[j], a[i];
+          assert prevASeq == a[..];
+          Swap(a, i, j);
+          i := i + 1;
+          assert Model.Shuffle(prevASeq, prevI)(prevS) == Model.Shuffle(a[..], i)(s) by {
+            calc {
+              Model.Shuffle(prevASeq, prevI)(prevS);
+              Model.Shuffle(Model.Swap(prevASeq, prevI, Uniform.Model.IntervalSample(prevI, |prevASeq|)(prevS).value), prevI + 1)(Uniform.Model.IntervalSample(prevI, |prevASeq|)(prevS).rest);
+              { assert Uniform.Model.IntervalSample(prevI, |prevASeq|)(prevS).value == j;
+                assert Uniform.Model.IntervalSample(prevI, |prevASeq|)(prevS).rest == s; }
+              Model.Shuffle(Model.Swap(prevASeq, prevI, j), prevI + 1)(s);
+              { assert i == prevI + 1;
+                assert Model.Swap(prevASeq, prevI, j) == a[..];
+              }
+              Model.Shuffle(a[..], i)(s);
+            }
+          }
         }
+
+        assert Model.Shuffle(old(a[..]))(old(s)) == Monad.Result(a[..], s) by {
+          assert i == a.Length - 1;
+          calc {
+            Model.Shuffle(old(a[..]))(old(s));
+            Model.Shuffle(prevASeq, prevI)(prevS);
+            Model.Shuffle(a[..], i)(s);
+            Monad.Return(a[..])(s);
+            Monad.Result(a[..], s);
+          }
+        }
+
       }
+    }
+
+    method Swap<T>(a: array<T>, i: nat, j: nat)
+      modifies a
+      requires i <= j
+      requires 0 <= i < a.Length
+      requires 0 <= j < a.Length
+      ensures Model.Swap(old(a[..]), i, j) == a[..]
+      ensures old(s) == s
+    {
+      a[i], a[j] := a[j], a[i];
     }
 
   }
